Weidenbach_Book/IsaSAT/Pointer_LLVM.thy
@@ -29,48 +29,49 @@ text \<open> In this theory we define a refinement relation to represent pointer
 definition pointer_assn :: \<open>('a \<Rightarrow> 'b::llvm_rep \<Rightarrow> llvm_amemory \<Rightarrow> bool) \<Rightarrow> 'a \<Rightarrow> 'b ptr \<Rightarrow> llvm_amemory \<Rightarrow> bool\<close> where
   \<open>pointer_assn R = assn_comp R (\<upharpoonleft>ll_bpto)\<close>
 
+definition ptr_read0 where
+  \<open>ptr_read0 f' a = f' a\<close>
+
+
+definition ptr_read0_code :: "_ \<Rightarrow> 'a::llvm_rep ptr \<Rightarrow> _" where
+  \<open>ptr_read0_code f a = doM {
+    b \<leftarrow> ll_load a;
+    f (b)
+  }\<close>
+
 context
   fixes f ::  "'a::llvm_rep \<Rightarrow> _" and  R P and f' and b_assn
   assumes [vcg_rules]: \<open>P x \<Longrightarrow>
   nofail (f' x) \<Longrightarrow> llvm_htriple (R x xi) (f xi) (\<lambda>r. R x xi \<and>* (\<lambda>s. \<exists>xa. (b_assn xa r \<and>* \<up>(RETURN xa \<le> f' x)) s))\<close>
 begin
 
-definition ptr_read where
-  \<open>ptr_read a = f' a\<close>
 
-
-definition ptr_read_code :: "'a::llvm_rep ptr \<Rightarrow> _" where
-  \<open>ptr_read_code a = doM {
-    b \<leftarrow> ll_load a;
-    f (b)
-  }\<close>
-
-lemma bpto_ptr_read_code: "nofail (f' ys) \<Longrightarrow> llvm_htriple
+lemma bpto_ptr_read0_code: "nofail (f' ys) \<Longrightarrow> llvm_htriple
   (\<upharpoonleft>ll_bpto xs p \<and>* R ys xs \<and>* \<up>\<^sub>d (P ys))
-  (ptr_read_code p)
-  (\<lambda>r. (\<lambda>s. \<exists>xa. (b_assn xa r \<and>* \<up>(RETURN xa \<le> ptr_read ys)) s) \<and>* \<upharpoonleft>ll_bpto xs p \<and>* (\<lambda>s. True))"  
-  unfolding ptr_read_code_def ptr_read_def
+  (ptr_read0_code f p)
+  (\<lambda>r. (\<lambda>s. \<exists>xa. (b_assn xa r \<and>* \<up>(RETURN xa \<le> ptr_read0 f' ys)) s) \<and>* \<upharpoonleft>ll_bpto xs p \<and>* (\<lambda>s. True))"  
+  unfolding ptr_read0_code_def ptr_read0_def
   apply vcg
   apply (auto simp: ENTAILS_def)
   by (smt (verit, del_insts) conj_entails_mono entails_def pure_true_conv sep.add.right_neutral sep_conj_left_commute)
 
-lemma bpto_ptr_read_code2: "nofail (f' ys) \<Longrightarrow> llvm_htriple
+lemma bpto_ptr_read0_code2: "nofail (f' ys) \<Longrightarrow> llvm_htriple
   (pointer_assn R ys p \<and>* \<up>\<^sub>d (P ys))
-  (ptr_read_code p)
-  (\<lambda>r. (\<lambda>s. \<exists>xa. (b_assn xa r \<and>* \<up>(RETURN xa \<le> ptr_read ys)) s) \<and>* pointer_assn R ys p)"  
-  unfolding ptr_read_code_def pointer_assn_def assn_comp_def ptr_read_def
+  (ptr_read0_code f p)
+  (\<lambda>r. (\<lambda>s. \<exists>xa. (b_assn xa r \<and>* \<up>(RETURN xa \<le> ptr_read0 f' ys)) s) \<and>* pointer_assn R ys p)"  
+  unfolding ptr_read0_code_def pointer_assn_def assn_comp_def ptr_read0_def
   apply vcg
   done
 end
 
 
-lemma no_fail_ptr_read_iff: \<open>nofail (ptr_read f' x) \<longleftrightarrow> nofail (f' x)\<close>
- by (auto simp: ptr_read_def)
+lemma no_fail_ptr_read0_iff: \<open>nofail (ptr_read0 f' x) \<longleftrightarrow> nofail (f' x)\<close>
+ by (auto simp: ptr_read0_def)
 
 lemma exists_eq_star_conv': "(\<lambda>s. (\<exists>x. (\<up>(x = k) \<and>* F x) s)) = F k"
   by (auto simp: sep_algebra_simps sep_conj_def pred_lift_extract_simps)
 
-locale ptr_read_loc =
+locale ptr_read0_loc =
   fixes f ::  "'a::llvm_rep \<Rightarrow> _" and f' and ptr_assn and b_assn and R and P
   assumes H: \<open>(f, f') \<in> [P]\<^sub>a (R)\<^sup>k \<rightarrow> b_assn\<close>
   notes [[sepref_register_adhoc f']]
@@ -78,11 +79,11 @@ locale ptr_read_loc =
 begin
 
 
-lemma ptr_read_code_rule:
+lemma ptr_read0_code_rule:
   assumes \<open>nofail (f' ys)\<close>
-  shows "llvm_htriple (pointer_assn R ys p \<and>* \<up>\<^sub>dP ys) (ptr_read_code f p)
- (\<lambda>r. (\<lambda>s. \<exists>xa. (b_assn xa r \<and>* \<up>(RETURN xa \<le> ptr_read f' ys)) s) \<and>* pointer_assn R ys p)"
-  apply (rule bpto_ptr_read_code2)
+  shows "llvm_htriple (pointer_assn R ys p \<and>* \<up>\<^sub>dP ys) (ptr_read0_code f p)
+ (\<lambda>r. (\<lambda>s. \<exists>xa. (b_assn xa r \<and>* \<up>(RETURN xa \<le> ptr_read0 f' ys)) s) \<and>* pointer_assn R ys p)"
+  apply (rule bpto_ptr_read0_code2)
   unfolding htriple_def
   apply (intro conjI impI allI)
   apply (rule wpa_monoI)
@@ -95,7 +96,87 @@ lemma ptr_read_code_rule:
 
 
 
-lemma ptr_read_code: \<open>(ptr_read_code f, ptr_read f') \<in> [P]\<^sub>a (pointer_assn R)\<^sup>k \<rightarrow> b_assn\<close>
+lemma refine: \<open>(ptr_read0_code f, ptr_read0 f') \<in> [P]\<^sub>a (pointer_assn R)\<^sup>k \<rightarrow> b_assn\<close>
+  supply [simp] = no_fail_ptr_read0_iff
+  supply [vcg_rules] = ptr_read0_code_rule
+  apply sepref_to_hoare
+  apply vcg
+  done
+
+end
+
+
+definition ptr_read where
+  \<open>ptr_read f' a b = f' a b\<close>
+
+
+definition ptr_read_code :: "_ \<Rightarrow> 'a::llvm_rep ptr \<Rightarrow> _" where
+  \<open>ptr_read_code f a c = doM {
+    b \<leftarrow> ll_load a;
+    f (b) c
+  }\<close>
+
+
+context
+  fixes f ::  "'a::llvm_rep \<Rightarrow> 'b :: llvm_rep \<Rightarrow> _" and  R and S P and f' and b_assn
+  assumes [vcg_rules]: \<open>P (x,y) \<Longrightarrow>
+  nofail (f' x y) \<Longrightarrow> llvm_htriple (R x xi \<and>* S y yi) (f xi yi) (\<lambda>r. R x xi \<and>* S y yi \<and>* (\<lambda>s. \<exists>xa. (b_assn xa r \<and>* \<up>(RETURN xa \<le> f' x y)) s))\<close>
+begin
+
+lemma bpto_ptr_read_code: "nofail (f' ys y) \<Longrightarrow> llvm_htriple
+  (\<upharpoonleft>ll_bpto xs p \<and>* R ys xs \<and>* S y yi \<and>* \<up>\<^sub>d (P (ys, y)))
+  (ptr_read_code f p yi)
+  (\<lambda>r.  (\<lambda>s. \<exists>xa. (b_assn xa r \<and>* \<up>(RETURN xa \<le> ptr_read f' ys y)) s) \<and>* \<upharpoonleft>ll_bpto xs p \<and>* S y yi \<and>* (\<lambda>_. True))"  
+  unfolding ptr_read_code_def ptr_read_def
+  apply vcg
+  apply (auto simp: ENTAILS_def sep_conj_commute sep_conj_left_commute[of _ \<open>S _ _\<close>])
+  apply (rule conj_entails_mono)
+  apply blast
+  apply (subst sep_conj_commute sep_conj_left_commute[of _ \<open>\<upharpoonleft>ll_bpto _ _\<close>])
+  apply (subst sep_conj_commute sep_conj_left_commute[of _ \<open>\<upharpoonleft>ll_bpto _ _\<close>])
+  unfolding sep.add_assoc
+  apply (rule conj_entails_mono)
+  apply blast
+  by (smt (verit, del_insts) conj_entails_mono entails_def pure_true_conv sep.add.right_neutral sep_conj_left_commute)
+
+lemma bpto_ptr_read_code2: "nofail (f' ys y) \<Longrightarrow> llvm_htriple
+  (pointer_assn R ys p \<and>* S y yi \<and>* \<up>\<^sub>d (P (ys, y)))
+  (ptr_read_code f p yi)
+  (\<lambda>r.  (\<lambda>s. \<exists>xa. (b_assn xa r \<and>* \<up>(RETURN xa \<le> ptr_read f' ys y)) s) \<and>* S y yi \<and>* pointer_assn R ys p)"  
+  unfolding ptr_read_code_def pointer_assn_def assn_comp_def ptr_read_def
+  apply vcg
+  done
+end
+
+
+lemma no_fail_ptr_read_iff: \<open>nofail (ptr_read f' x y) \<longleftrightarrow> nofail (f' x y)\<close>
+ by (auto simp: ptr_read_def)
+
+locale ptr_read_loc =
+  fixes f ::  "'a::llvm_rep \<Rightarrow> _ :: llvm_rep \<Rightarrow> _" and f' and ptr_assn and b_assn and R and P and S
+  assumes H: \<open>(uncurry f, uncurry f') \<in> [P]\<^sub>a (R)\<^sup>k *\<^sub>a S\<^sup>k \<rightarrow> b_assn\<close>
+  notes [[sepref_register_adhoc f']]
+  notes [fcomp_norm_unfold] = pointer_assn_def[symmetric]
+begin
+
+lemma ptr_read_code_rule:
+  assumes \<open>nofail (f' ys y)\<close>
+  shows "llvm_htriple (pointer_assn R ys p \<and>* S y yi \<and>* \<up>\<^sub>dP (ys, y)) (ptr_read_code f p yi)
+ (\<lambda>r. (\<lambda>s. \<exists>xa. (b_assn xa r \<and>*  \<up>(RETURN xa \<le> ptr_read f' ys y)) s) \<and>*  S y yi \<and>* pointer_assn R ys p)"
+  apply (rule bpto_ptr_read_code2)
+  unfolding htriple_def
+  apply (intro conjI impI allI)
+  apply (rule wpa_monoI)
+    thm H[to_hnr, simplified, unfolded hn_ctxt_def hn_refine_def htriple_def
+    sep_conj_empty' pure_true_conv sep.add_assoc, rule_format]
+  apply (rule H[to_hnr, simplified, unfolded hn_ctxt_def hn_refine_def htriple_def
+    sep_conj_empty' pure_true_conv sep.add_assoc, rule_format])
+  apply assumption
+  apply assumption
+  apply (auto simp: pure_def exists_eq_star_conv' assms)
+  done
+
+lemma refine: \<open>(uncurry (ptr_read_code f), uncurry (ptr_read f')) \<in> [P]\<^sub>a (pointer_assn R)\<^sup>k *\<^sub>a S\<^sup>k \<rightarrow> b_assn\<close>
   supply [simp] = no_fail_ptr_read_iff
   supply [vcg_rules] = ptr_read_code_rule
   apply sepref_to_hoare
@@ -105,29 +186,92 @@ lemma ptr_read_code: \<open>(ptr_read_code f, ptr_read f') \<in> [P]\<^sub>a (po
 end
 
 
+definition ptr_read2 where
+  \<open>ptr_read2 f' a b c = f' a b c\<close>
+
+
+definition ptr_read2_code :: "_ \<Rightarrow> 'a::llvm_rep ptr \<Rightarrow> _" where
+  \<open>ptr_read2_code f a c d = doM {
+    b \<leftarrow> ll_load a;
+    f (b) c d
+  }\<close>
+
+locale ptr_read2_loc =
+  fixes f ::  "'a::llvm_rep \<Rightarrow> _ :: llvm_rep \<Rightarrow>_ :: llvm_rep \<Rightarrow> _" and f' and ptr_assn and b_assn and R and P and S and T
+  assumes H: \<open>(uncurry2 f, uncurry2 f') \<in> [P]\<^sub>a (R)\<^sup>k *\<^sub>a S\<^sup>k *\<^sub>a T\<^sup>k \<rightarrow> b_assn\<close>
+  notes [[sepref_register_adhoc f']]
+  notes [fcomp_norm_unfold] = pointer_assn_def[symmetric]
+begin
+
+sublocale XX: ptr_read_loc where
+  f = \<open>\<lambda>a (b,c). f a b c\<close> and
+  f' = \<open>\<lambda>a (b,c). f' a b c\<close> and
+  P = \<open>\<lambda>(a, (b,c)). P ((a,b), c)\<close> and
+  S = \<open>S \<times>\<^sub>a T\<close>
+  by unfold_locales
+   (use H in \<open>simp add: hfref_def\<close>)
+
+lemma refine: \<open>(uncurry2 (ptr_read2_code f), uncurry2 (ptr_read2 f')) \<in> [P]\<^sub>a (pointer_assn R)\<^sup>k *\<^sub>a S\<^sup>k *\<^sub>a T\<^sup>k \<rightarrow> b_assn\<close>
+  by (use XX.refine in \<open>simp add: hfref_def ptr_read_code_def ptr_read2_code_def
+    ptr_read_def ptr_read2_def\<close>)
+
+end
+
+
+definition ptr_read3 where
+  \<open>ptr_read3 f' a b c d = f' a b c d\<close>
+
+
+definition ptr_read3_code :: "_ \<Rightarrow> 'a::llvm_rep ptr \<Rightarrow> _" where
+  \<open>ptr_read3_code f a c d e = doM {
+    b \<leftarrow> ll_load a;
+    f (b) c d e
+  }\<close>
+
+locale ptr_read3_loc =
+  fixes f ::  "'a::llvm_rep \<Rightarrow> _ :: llvm_rep \<Rightarrow>_ :: llvm_rep \<Rightarrow> _ :: llvm_rep \<Rightarrow>  _" and f' and
+    ptr_assn and b_assn and R and P and S and T and U
+  assumes H: \<open>(uncurry3 f, uncurry3 f') \<in> [P]\<^sub>a (R)\<^sup>k *\<^sub>a S\<^sup>k *\<^sub>a T\<^sup>k *\<^sub>a U\<^sup>k \<rightarrow> b_assn\<close>
+  notes [[sepref_register_adhoc f']]
+  notes [fcomp_norm_unfold] = pointer_assn_def[symmetric]
+begin
+
+sublocale XX: ptr_read_loc where
+  f = \<open>\<lambda>a (b,c,d). f a b c d\<close> and
+  f' = \<open>\<lambda>a (b,c,d). f' a b c d\<close> and
+  P = \<open>\<lambda>(a, (b,c,d)). P (((a,b), c), d)\<close> and
+  S = \<open>S \<times>\<^sub>a T \<times>\<^sub>a U\<close>
+  by unfold_locales
+   (use H in \<open>simp add: hfref_def\<close>)
+
+lemma refine: \<open>(uncurry3 (ptr_read3_code f), uncurry3 (ptr_read3 f')) \<in> [P]\<^sub>a (pointer_assn R)\<^sup>k *\<^sub>a S\<^sup>k *\<^sub>a T\<^sup>k*\<^sub>a U\<^sup>k \<rightarrow> b_assn\<close>
+  by (use XX.refine in \<open>simp add: hfref_def ptr_read_code_def ptr_read3_code_def
+    ptr_read_def ptr_read3_def\<close>)
+
+end
+
+
+definition ptr_write0 where
+  \<open>ptr_write0 f' a = f' a\<close>
+
+definition ptr_write_code0 :: "_ \<Rightarrow> 'a::llvm_rep ptr \<Rightarrow> ('e \<times> 'a ptr) llM" where
+  \<open>ptr_write_code0 f a = doM {
+    b \<leftarrow> ll_load a;
+    (d, c) \<leftarrow> f (b);
+    ll_store c a;
+    Mreturn (d, a)
+  }\<close>
 
 context
   fixes f ::  "'a::llvm_rep \<Rightarrow> _" and  R P and f' and b_assn and S
   assumes writer_rule: \<open>P x \<Longrightarrow>
-  nofail (f' x) \<Longrightarrow> llvm_htriple (R x xi) (f xi) (\<lambda>r. (\<lambda>s. \<exists>xa xb. (R xa (fst r) \<and>* S xb (snd r) \<and>* \<up>(RETURN (xa, xb) \<le> f' x)) s) \<and>* \<box>)\<close>
+  nofail (f' x) \<Longrightarrow> llvm_htriple (R x xi) (f xi) (\<lambda>r. (\<lambda>s. \<exists>xa xb. (S xa (fst r) \<and>* R xb (snd r) \<and>* \<up>(RETURN (xa, xb) \<le> f' x)) s) \<and>* \<box>)\<close>
 begin
-
-definition ptr_write0 where
-  \<open>ptr_write0 a = f' a\<close>
-
-
-definition ptr_write_code0 :: "'a::llvm_rep ptr \<Rightarrow> ('a ptr \<times> 'e) llM" where
-  \<open>ptr_write_code0 a = doM {
-    b \<leftarrow> ll_load a;
-    (c, d) \<leftarrow> f (b);
-    ll_store c a;
-    Mreturn (a, d)
-  }\<close>
 
 lemma bpto_ptr_write_code2: "nofail (f' ys) \<Longrightarrow> llvm_htriple
   (pointer_assn R ys p \<and>* \<up>\<^sub>d (P ys))
-  (ptr_write_code0 p)
-  (\<lambda>r. (\<lambda>s. \<exists>xa xb. (pointer_assn R xa (fst r) \<and>* S xb (snd r) \<and>* \<up>(RETURN (xa, xb) \<le> ptr_write0 ys)) s) \<and>* \<box>)"
+  (ptr_write_code0 f p)
+  (\<lambda>r. (\<lambda>s. \<exists>xa xb. (S xa (fst r) \<and>* pointer_assn R xb (snd r) \<and>* \<up>(RETURN (xa, xb) \<le> ptr_write0 f' ys)) s) \<and>* \<box>)"
   supply [vcg_rules] = writer_rule
   unfolding ptr_write_code0_def pointer_assn_def assn_comp_def ptr_write0_def
   apply vcg
@@ -140,7 +284,7 @@ lemma [simp]: \<open>nofail (ptr_write0 f' x) \<longleftrightarrow> nofail (f' x
 
 locale ptr_write_loc0 =
   fixes f ::  "'a::llvm_rep \<Rightarrow> _" and f' and ptr_assn and b_assn and R and P and S
-  assumes H: \<open>(f, f') \<in> [P]\<^sub>a (R)\<^sup>d \<rightarrow> R \<times>\<^sub>a S\<close>
+  assumes H: \<open>(f, f') \<in> [P]\<^sub>a (R)\<^sup>d \<rightarrow> S \<times>\<^sub>a R\<close>
   notes [[sepref_register_adhoc f']]
   notes [fcomp_norm_unfold] = pointer_assn_def[symmetric]
 begin
@@ -148,7 +292,7 @@ begin
 lemma ptr_write_code_rule:
   assumes \<open>nofail (f' ys)\<close>
   shows "llvm_htriple (pointer_assn R ys p \<and>* \<up>\<^sub>dP ys) (ptr_write_code0 f p)
-    (\<lambda>r. (\<lambda>s. \<exists>xa xb. (pointer_assn R xa (fst r) \<and>*  S xb (snd r) \<and>* \<up>(RETURN (xa, xb) \<le> ptr_write0 f' ys)) s) \<and>* \<box>)"
+    (\<lambda>r. (\<lambda>s. \<exists>xa xb. (S xa (fst r) \<and>*  pointer_assn R xb (snd r) \<and>* \<up>(RETURN (xa, xb) \<le> ptr_write0 f' ys)) s) \<and>* \<box>)"
   (*supply [vcg_rules] = bpto_ptr_write_code2 does not work it looses track of dependencies between variables*)
   apply vcg
   apply (subst POSTCOND_def)
@@ -170,7 +314,7 @@ defer
   apply assumption
   by (simp add: STATE_extract(2) invalid_assn_def pure_true_conv)
 
-lemma ptr_write_code: \<open>(ptr_write_code0 f, ptr_write0 f') \<in> [P]\<^sub>a (pointer_assn R)\<^sup>d \<rightarrow> pointer_assn R \<times>\<^sub>a S\<close>
+lemma refine: \<open>(ptr_write_code0 f, ptr_write0 f') \<in> [P]\<^sub>a (pointer_assn R)\<^sup>d \<rightarrow> S \<times>\<^sub>a pointer_assn R\<close>
   supply [vcg_rules] = ptr_write_code_rule
   apply sepref_to_hoare
   apply vcg
@@ -182,36 +326,39 @@ end
 
 context
   fixes
-    f :: \<open>'a::llvm_rep \<Rightarrow> 'b :: llvm_rep \<Rightarrow> ('a \<times> 'cc) llM\<close> and
-    R :: \<open>'a2 \<Rightarrow> 'a \<Rightarrow> _\<close> and
-    S :: \<open>'b2 \<Rightarrow> 'b \<Rightarrow> _\<close> and
+    f :: \<open>'a::llvm_rep \<Rightarrow> 'b :: llvm_rep \<Rightarrow> ('cc \<times> 'a) llM\<close> and
+    R :: \<open>'a2 \<Rightarrow> 'a \<Rightarrow> llvm_amemory \<Rightarrow> bool\<close> and
+    S :: \<open>'b2 \<Rightarrow> 'b \<Rightarrow> llvm_amemory \<Rightarrow> bool\<close> and
     T :: \<open>'cc2 \<Rightarrow> 'cc \<Rightarrow> llvm_amemory \<Rightarrow> bool\<close> and
-    P :: \<open>'a2 \<Rightarrow> 'b2 \<Rightarrow> bool\<close> and
-    f' :: \<open>'a2 \<Rightarrow> 'b2 \<Rightarrow> ('a2 \<times> 'cc2) nres\<close> 
-  assumes writer_rule: \<open>P x a \<Longrightarrow>
-  nofail (f' x a) \<Longrightarrow> llvm_htriple (R x xi \<and>* S a b) (f xi b) (\<lambda>r. S a b \<and>* (\<lambda>s. \<exists>xa xb. (R xa (fst r) \<and>* T xb (snd r) \<and>* \<up>(RETURN (xa, xb) \<le> f' x a)) s))\<close>
+    P :: \<open>'a2 \<times> 'b2 \<Rightarrow> bool\<close> and
+    f' :: \<open>'a2 \<Rightarrow> 'b2 \<Rightarrow> ('cc2 \<times> 'a2) nres\<close> 
 begin
 definition ptr_write where
   \<open>ptr_write a b = f' a b\<close>
 
 
-definition ptr_write_code :: "'a::llvm_rep ptr \<Rightarrow> _ \<Rightarrow> ('a ptr \<times> 'cc) llM" where
+definition ptr_write_code :: "'a::llvm_rep ptr \<Rightarrow> 'b \<Rightarrow>  ('cc \<times> 'a ptr) llM" where
   \<open>ptr_write_code a d = doM {
     b \<leftarrow> ll_load a;
-    (c, d) \<leftarrow> f (b) d;
+    (d, c) \<leftarrow> f (b) d;
     ll_store c a;
-    Mreturn (a, d)
+    Mreturn (d, a)
   }\<close>
 
+context
+  assumes writer_rule: \<open>P (x, a) \<Longrightarrow>
+  nofail (f' x a) \<Longrightarrow> llvm_htriple (R x xi \<and>* S a b) (f xi b) (\<lambda>r. S a b \<and>* (\<lambda>s. \<exists>xa xb. (T xa (fst r) \<and>* R xb (snd r) \<and>* \<up>(RETURN (xa, xb) \<le> f' x a)) s))\<close>
+begin
+
 lemma bpto_ptr_write_code: "nofail (f' ys a) \<Longrightarrow> llvm_htriple
-  (pointer_assn R ys p \<and>* S a b \<and>* \<up>\<^sub>d (P ys a))
+  (pointer_assn R ys p \<and>* S a b \<and>* \<up>\<^sub>d P (ys, a))
   (ptr_write_code p b)
-  (\<lambda>r. S a b \<and>* (\<lambda>s. \<exists>xa xb. (pointer_assn R xa (fst r) \<and>* T xb (snd r) \<and>* \<up>(RETURN (xa, xb) \<le> ptr_write ys a)) s))"
+  (\<lambda>r. S a b \<and>* (\<lambda>s. \<exists>xa xb. (T xa (fst r) \<and>* pointer_assn R xb (snd r) \<and>* \<up>(RETURN (xa, xb) \<le> ptr_write ys a)) s))"
   supply [vcg_rules] = writer_rule
   unfolding ptr_write_code_def pointer_assn_def assn_comp_def ptr_write_def
   apply vcg
   done
-
+end
 end
 
 lemma [simp]: \<open>nofail (ptr_write f' x a) \<longleftrightarrow> nofail (f' x a)\<close>
@@ -219,13 +366,13 @@ lemma [simp]: \<open>nofail (ptr_write f' x a) \<longleftrightarrow> nofail (f' 
 
 locale ptr_write_loc =
   fixes
-    f :: \<open>'a::llvm_rep \<Rightarrow> 'b :: llvm_rep \<Rightarrow> ('a \<times> 'cc) llM\<close> and
+    f :: \<open>'a :: llvm_rep \<Rightarrow> 'b::llvm_rep \<Rightarrow> ('cc \<times> 'a) llM\<close> and
     R :: \<open>'a2 \<Rightarrow> 'a \<Rightarrow> _\<close> and
     S :: \<open>'b2 \<Rightarrow> 'b \<Rightarrow> _\<close> and
     T :: \<open>'cc2 \<Rightarrow> 'cc \<Rightarrow> llvm_amemory \<Rightarrow> bool\<close> and
-    P :: \<open>'a2 \<Rightarrow> 'b2 \<Rightarrow> bool\<close> and
-    f' :: \<open>'a2 \<Rightarrow> 'b2 \<Rightarrow> ('a2 \<times> 'cc2) nres\<close> 
-  assumes H: \<open>(uncurry f, uncurry f') \<in> [uncurry P]\<^sub>a (R)\<^sup>d *\<^sub>a S\<^sup>k \<rightarrow> R \<times>\<^sub>a T\<close>
+    P :: \<open>'a2 \<times> 'b2 \<Rightarrow> bool\<close> and
+    f' :: \<open>'a2 \<Rightarrow>'b2 \<Rightarrow>  ('cc2 \<times> 'a2) nres\<close> 
+  assumes H: \<open>(uncurry f, uncurry f') \<in> [P]\<^sub>a (R)\<^sup>d *\<^sub>a S\<^sup>k \<rightarrow> T \<times>\<^sub>a R\<close>
   notes [[sepref_register_adhoc f']]
   notes [fcomp_norm_unfold] = pointer_assn_def[symmetric]
 begin
@@ -233,8 +380,8 @@ begin
 lemma ptr_write_code_rule:
   fixes a b
   assumes \<open>nofail (f' ys a)\<close>
-   shows "llvm_htriple (pointer_assn R ys p \<and>* S a b \<and>* \<up>\<^sub>dP ys a) (ptr_write_code f p b)
-    (\<lambda>r.  S a b \<and>* (\<lambda>s. \<exists>xa xb. (pointer_assn R xa (fst r) \<and>*  T xb (snd r) \<and>* \<up>(RETURN (xa, xb) \<le> ptr_write f' ys a)) s))"
+   shows "llvm_htriple (pointer_assn R ys p \<and>* S a b \<and>* \<up>\<^sub>dP (ys, a)) (ptr_write_code f p b)
+    (\<lambda>r.  S a b \<and>* (\<lambda>s. \<exists>xa xb. (T xa (fst r) \<and>*  pointer_assn R xb (snd r) \<and>* \<up>(RETURN (xa, xb) \<le> ptr_write f' ys a)) s))"
   (*supply [vcg_rules] = bpto_ptr_write_code2 does not work it looses track of dependencies between variables*)
   unfolding pure_true_conv sep_conj_empty'
   apply vcg
@@ -255,9 +402,10 @@ defer
   apply (auto simp: pure_def exists_eq_star_conv' assms)
   apply (rule STATE_monoI)
   apply assumption
-  by (simp add: STATE_extract(2) invalid_assn_def pure_true_conv)
+  by (simp add: STATE_extract(2) invalid_assn_def pure_true_conv sep_algebra_class.sep_conj_commute
+    conj_entails_mono entails_lift_extract_simps(2))
 
-lemma refine: \<open>(uncurry (ptr_write_code f), uncurry (ptr_write f')) \<in> [uncurry P]\<^sub>a (pointer_assn R)\<^sup>d *\<^sub>a S\<^sup>k \<rightarrow> pointer_assn R \<times>\<^sub>a T\<close>
+lemma refine: \<open>(uncurry (ptr_write_code f), uncurry (ptr_write f')) \<in> [P]\<^sub>a (pointer_assn R)\<^sup>d *\<^sub>a S\<^sup>k\<rightarrow> T \<times>\<^sub>a pointer_assn R\<close>
   supply [vcg_rules] = ptr_write_code_rule
   apply sepref_to_hoare
   unfolding pure_true_conv sep_conj_empty'
@@ -267,70 +415,167 @@ lemma refine: \<open>(uncurry (ptr_write_code f), uncurry (ptr_write f')) \<in> 
 end
 
 
+context
+  fixes
+    f :: \<open>'b :: llvm_rep \<Rightarrow> 'a::llvm_rep \<Rightarrow> ('a) llM\<close> and
+    R :: \<open>'a2 \<Rightarrow> 'a \<Rightarrow> llvm_amemory \<Rightarrow> bool\<close> and
+    S :: \<open>'b2 \<Rightarrow> 'b \<Rightarrow> llvm_amemory \<Rightarrow> bool\<close> and
+    P :: \<open>'b2 \<times> 'a2 \<Rightarrow> bool\<close> and
+    f' :: \<open>'b2 \<Rightarrow> 'a2 \<Rightarrow> ('a2) nres\<close> 
+begin
+
+definition ptr_write_inplace where
+  \<open>ptr_write_inplace a b = f' a b\<close>
+
+
+definition ptr_write_inplace_code :: "'b \<Rightarrow> 'a::llvm_rep ptr \<Rightarrow>  ('a ptr) llM" where
+  \<open>ptr_write_inplace_code d a = doM {
+    b \<leftarrow> ll_load a;
+    c \<leftarrow> f d (b);
+    ll_store c a;
+    Mreturn (a)
+  }\<close>
+
+context
+  assumes writer_rule: \<open>P (a, x) \<Longrightarrow>
+  nofail (f' a x) \<Longrightarrow> llvm_htriple (R x xi \<and>* S a b) (f b xi) (\<lambda>r.  (\<lambda>s. \<exists>xa. (R xa (r) \<and>* \<up>(RETURN (xa) \<le> f' a x)) s))\<close>
+begin
+
+lemma bpto_ptr_write_inplace_code: "nofail (f' a ys) \<Longrightarrow> llvm_htriple
+  (pointer_assn R ys p \<and>* S a b \<and>* \<up>\<^sub>d P (a, ys))
+  (ptr_write_inplace_code b p)
+  (\<lambda>r.  (\<lambda>s. \<exists>xa. (pointer_assn R xa (r) \<and>* \<up>(RETURN (xa) \<le> ptr_write_inplace a ys)) s))"
+  supply [vcg_rules] = writer_rule
+  unfolding ptr_write_inplace_code_def pointer_assn_def assn_comp_def ptr_write_inplace_def
+  apply vcg
+  done
+
+end
+
+end
+
+lemma [simp]: \<open>nofail (ptr_write_inplace f' x a) \<longleftrightarrow> nofail (f' x a)\<close>
+  by (auto simp: ptr_write_inplace_def)
+
+
+locale ptr_write_loc_inplace =
+  fixes
+    f :: \<open>'b::llvm_rep \<Rightarrow> 'a :: llvm_rep \<Rightarrow> ('a) llM\<close> and
+    R :: \<open>'a2 \<Rightarrow> 'a \<Rightarrow> _\<close> and
+    S :: \<open>'b2 \<Rightarrow> 'b \<Rightarrow> _\<close> and
+    P :: \<open>'b2 \<times> 'a2 \<Rightarrow> bool\<close> and
+    f' :: \<open>'b2 \<Rightarrow> 'a2 \<Rightarrow> ('a2) nres\<close> 
+  assumes H: \<open>(uncurry f, uncurry f') \<in> [P]\<^sub>a S\<^sup>d *\<^sub>a (R)\<^sup>d \<rightarrow> R\<close>
+  notes [[sepref_register_adhoc f']]
+  notes [fcomp_norm_unfold] = pointer_assn_def[symmetric]
+begin
+
+
+lemma ptr_write_code_rule:
+  fixes a b
+  assumes \<open>nofail (f' a ys)\<close>
+   shows "llvm_htriple (pointer_assn R ys p \<and>* S a b \<and>* \<up>\<^sub>dP (a, ys)) (ptr_write_inplace_code f b p)
+    (\<lambda>r.  (\<lambda>s. \<exists>xa. (pointer_assn R xa ( r) \<and>*  \<up>(RETURN (xa) \<le> ptr_write_inplace f' a ys)) s))"
+  (*supply [vcg_rules] = bpto_ptr_write_code2 does not work it looses track of dependencies between variables*)
+  unfolding pure_true_conv sep_conj_empty'
+  apply vcg
+  apply (subst POSTCOND_def)
+  apply (rule bpto_ptr_write_inplace_code[simplified, unfolded hn_ctxt_def hn_refine_def htriple_def
+    sep_conj_empty' pure_true_conv sep.add_assoc, rule_format, where P=P])
+defer
+ apply (rule assms)
+ apply (auto simp: pure_def exists_eq_star_conv' assms SOLVE_AUTO_DEFER_def
+     pure_true_conv)[]
+
+  apply (rule wpa_monoI)
+  apply (rule H[to_hnr, simplified, unfolded hn_ctxt_def hn_refine_def htriple_def
+    sep_conj_empty' pure_true_conv sep.add_assoc, rule_format])
+  apply assumption back
+  apply assumption
+  apply (subst sep_conj_commute)
+  apply assumption
+  apply (auto simp: pure_def exists_eq_star_conv' assms)
+  apply (rule STATE_monoI)
+  apply assumption
+  by (simp add: STATE_extract(2) invalid_assn_def pure_true_conv sep_algebra_class.sep_conj_commute
+    conj_entails_mono entails_lift_extract_simps(2))
+
+lemma refine: \<open>(uncurry (ptr_write_inplace_code f), uncurry (ptr_write_inplace f')) \<in> [P]\<^sub>a S\<^sup>d *\<^sub>a (pointer_assn R)\<^sup>d \<rightarrow> pointer_assn R\<close>
+  supply [vcg_rules] = ptr_write_code_rule
+  apply sepref_to_hoare
+  unfolding pure_true_conv sep_conj_empty'
+  apply vcg
+  done
+
+end
+
 definition ptr_write2 where
   \<open>ptr_write2 f' a b c = f' a b c\<close>
 
 
-definition ptr_write_code2 :: "_ \<Rightarrow> 'a::llvm_rep ptr \<Rightarrow> _ \<Rightarrow> _ \<Rightarrow> ('a ptr \<times> 'cc) llM" where
-  \<open>ptr_write_code2 f a d e = doM {
+definition ptr_write_code2 :: "_ \<Rightarrow>  _ \<Rightarrow> _ \<Rightarrow> 'a::llvm_rep ptr \<Rightarrow> ('cc \<times> 'a ptr) llM" where
+  \<open>ptr_write_code2 f d e a = doM {
     b \<leftarrow> ll_load a;
-    (c, d) \<leftarrow> f (b) d e;
+    (d, c) \<leftarrow> f d e b;
     ll_store c a;
-    Mreturn (a, d)
+    Mreturn (d, a)
   }\<close>
 
 locale ptr_write_loc2 =
   fixes
-    f :: \<open>'a::llvm_rep \<Rightarrow> 'b :: llvm_rep \<Rightarrow> 'c :: llvm_rep \<Rightarrow> ('a \<times> 'cc) llM\<close> and
+    f :: \<open>'b :: llvm_rep \<Rightarrow> 'c :: llvm_rep \<Rightarrow> 'a::llvm_rep \<Rightarrow> ('cc \<times> 'a) llM\<close> and
     R :: \<open>'a2 \<Rightarrow> 'a \<Rightarrow> _\<close> and
     S :: \<open>'b2 \<Rightarrow> 'b \<Rightarrow> _\<close> and
     T :: \<open>'c2 \<Rightarrow> 'c \<Rightarrow> _\<close> and
     U :: \<open>'cc2 \<Rightarrow> 'cc \<Rightarrow> llvm_amemory \<Rightarrow> bool\<close> and
-    P :: \<open>'a2 \<Rightarrow> 'b2 \<Rightarrow> 'c2 \<Rightarrow> bool\<close> and
-    f' :: \<open>'a2 \<Rightarrow> 'b2 \<Rightarrow> 'c2 \<Rightarrow> ('a2 \<times> 'cc2) nres\<close> 
-  assumes H: \<open>(uncurry2 f, uncurry2 f') \<in> [uncurry2 P]\<^sub>a (R)\<^sup>d *\<^sub>a S\<^sup>k *\<^sub>a T\<^sup>k \<rightarrow> R \<times>\<^sub>a U\<close>
+    P :: \<open>('b2 \<times> 'c2) \<times> 'a2 \<Rightarrow> bool\<close> and
+    f' :: \<open>'b2 \<Rightarrow> 'c2 \<Rightarrow> 'a2 \<Rightarrow> ('cc2 \<times> 'a2) nres\<close> 
+  assumes H: \<open>(uncurry2 f, uncurry2 f') \<in> [P]\<^sub>a S\<^sup>k *\<^sub>a T\<^sup>k *\<^sub>a R\<^sup>d \<rightarrow> U \<times>\<^sub>a R\<close>
   notes [[sepref_register_adhoc f']]
   notes [fcomp_norm_unfold] = pointer_assn_def[symmetric]
 begin
 
 sublocale XX: ptr_write_loc where
-  f = \<open>\<lambda>a (b,c). f a b c\<close> and
-  f' = \<open>\<lambda>a (b,c). f' a b c\<close> and
+  f = \<open>\<lambda>a (b,c). f b c a\<close> and
+  f' = \<open>\<lambda>a (b,c). f' b c a\<close> and
   R=R and
   S = \<open>S \<times>\<^sub>a T\<close> and
   T = U and
-  P =  \<open>\<lambda>a (b,c). P a b c\<close>
+  P =  \<open>\<lambda>(a, (b,c)). P ((b,c), a)\<close>
   by unfold_locales
-   (use H in \<open>simp add: hfref_def\<close>)
+   (use H in \<open>auto simp add: hfref_def sep_conj_commute\<close>)
 
 
-lemma refine: \<open>(uncurry2 (ptr_write_code2 f), uncurry2 (ptr_write2 f')) \<in> [uncurry2 P]\<^sub>a (pointer_assn R)\<^sup>d *\<^sub>a S\<^sup>k *\<^sub>a T\<^sup>k \<rightarrow> pointer_assn R \<times>\<^sub>a U\<close>
-  by (use XX.refine in \<open>auto simp add: hfref_def ptr_write2_def ptr_write_def ptr_write_code2_def ptr_write_code_def\<close>)
+lemma refine: \<open>(uncurry2 (ptr_write_code2 f), uncurry2 (ptr_write2 f')) \<in> [P]\<^sub>a S\<^sup>k *\<^sub>a T\<^sup>k *\<^sub>a (pointer_assn R)\<^sup>d \<rightarrow> U \<times>\<^sub>a pointer_assn R\<close>
+  by (use XX.refine in \<open>auto simp add: hfref_def ptr_write2_def ptr_write_def ptr_write_code2_def ptr_write_code_def
+    sep_conj_commute\<close>)
 
 end
 
+
+definition ptr_update0 where
+  \<open>ptr_update0 f' a = f' a\<close>
+
+
+definition ptr_update_code0 :: "_ \<Rightarrow> 'a::llvm_rep ptr \<Rightarrow> ('a ptr) llM" where
+  \<open>ptr_update_code0 f a = doM {
+    b \<leftarrow> ll_load a;
+    c \<leftarrow> f (b);
+    ll_store c a;
+    Mreturn (a)
+  }\<close>
+ 
 context
   fixes f ::  "'a::llvm_rep \<Rightarrow> _" and  R P and f' and b_assn and S
   assumes updater_rule: \<open>P x \<Longrightarrow>
   nofail (f' x) \<Longrightarrow> llvm_htriple (R x xi) (f xi) (\<lambda>r. (\<lambda>s. \<exists>xa xb. (R xa r \<and>* \<up>(RETURN (xa) \<le> f' x)) s) \<and>* \<box>)\<close>
 begin
 
-definition ptr_update0 where
-  \<open>ptr_update0 a = f' a\<close>
-
-
-definition ptr_update_code0 :: "'a::llvm_rep ptr \<Rightarrow> ('a ptr) llM" where
-  \<open>ptr_update_code0 a = doM {
-    b \<leftarrow> ll_load a;
-    c \<leftarrow> f (b);
-    ll_store c a;
-    Mreturn (a)
-  }\<close>
 
 lemma bpto_ptr_update_code2: "nofail (f' ys) \<Longrightarrow> llvm_htriple
   (pointer_assn R ys p \<and>* \<up>\<^sub>d (P ys))
-  (ptr_update_code0 p)
-  (\<lambda>r. (\<lambda>s. \<exists>xa xb. (pointer_assn R xa r \<and>* \<up>(RETURN (xa) \<le> ptr_update0 ys)) s) \<and>* \<box>)"
+  (ptr_update_code0 f p)
+  (\<lambda>r. (\<lambda>s. \<exists>xa xb. (pointer_assn R xa r \<and>* \<up>(RETURN (xa) \<le> ptr_update0 f' ys)) s) \<and>* \<box>)"
   supply [vcg_rules] = updater_rule
   unfolding ptr_update_code0_def pointer_assn_def assn_comp_def ptr_update0_def
   apply vcg
@@ -382,28 +627,29 @@ lemma ptr_update_hnr: \<open>(ptr_update_code0 f, ptr_update0 f') \<in> [P]\<^su
 end
 
 
-context
-  fixes f ::  "'a::llvm_rep \<Rightarrow> _" and  R P and f' and b_assn and S
-  assumes updater_rule: \<open>P x a \<Longrightarrow>
-  nofail (f' x a) \<Longrightarrow> llvm_htriple (R x xi \<and>* S a ai) (f xi ai) (\<lambda>r. (\<lambda>s. \<exists>xa xb. (R xa r \<and>* \<up>(RETURN (xa) \<le> f' x a)) s) \<and>* \<box>)\<close>
-begin
-
 definition ptr_update where
-  \<open>ptr_update a = f' a\<close>
+  \<open>ptr_update f' a = f' a\<close>
 
 
-definition ptr_update_code :: "'a::llvm_rep ptr \<Rightarrow> _ \<Rightarrow> ('a ptr) llM" where
-  \<open>ptr_update_code a d = doM {
+definition ptr_update_code :: "_ \<Rightarrow> 'a::llvm_rep ptr \<Rightarrow> _ \<Rightarrow> ('a ptr) llM" where
+  \<open>ptr_update_code f a d = doM {
     b \<leftarrow> ll_load a;
     c \<leftarrow> f (b) d;
     ll_store c a;
     Mreturn (a)
   }\<close>
 
+context
+  fixes f ::  "'a::llvm_rep \<Rightarrow> _" and  R P and f' and b_assn and S
+  assumes updater_rule: \<open>P (x, a) \<Longrightarrow>
+  nofail (f' x a) \<Longrightarrow> llvm_htriple (R x xi \<and>* S a ai) (f xi ai) (\<lambda>r. (\<lambda>s. \<exists>xa xb. (R xa r \<and>* \<up>(RETURN (xa) \<le> f' x a)) s) \<and>* \<box>)\<close>
+begin
+
+
 lemma bpto_ptr_update_code: "nofail (f' ys a) \<Longrightarrow> llvm_htriple
-  (pointer_assn R ys p \<and>* S a ai \<and>* \<up>\<^sub>d (P ys a))
-  (ptr_update_code p ai)
-  (\<lambda>r. (\<lambda>s. \<exists>xa xb. (pointer_assn R xa r \<and>* \<up>(RETURN (xa) \<le> ptr_update ys a)) s) \<and>* \<box>)"
+  (pointer_assn R ys p \<and>* S a ai \<and>* \<up>\<^sub>d P (ys, a))
+  (ptr_update_code f p ai)
+  (\<lambda>r. (\<lambda>s. \<exists>xa xb. (pointer_assn R xa r \<and>* \<up>(RETURN (xa) \<le> ptr_update f' ys a)) s) \<and>* \<box>)"
   supply [vcg_rules] = updater_rule
   unfolding ptr_update_code_def pointer_assn_def assn_comp_def ptr_update_def
   apply vcg
@@ -417,13 +663,13 @@ lemma [simp]: \<open>nofail (ptr_update f' x a) \<longleftrightarrow> nofail (f'
 
 locale ptr_update_loc =
   fixes f ::  "'a::llvm_rep \<Rightarrow> _ :: llvm_rep \<Rightarrow> _" and f' and ptr_assn and b_assn and R and P and S
-  assumes H: \<open>(uncurry f, uncurry f') \<in> [uncurry P]\<^sub>a (R)\<^sup>d *\<^sub>a S\<^sup>d \<rightarrow> R\<close>
+  assumes H: \<open>(uncurry f, uncurry f') \<in> [P]\<^sub>a (R)\<^sup>d *\<^sub>a S\<^sup>d \<rightarrow> R\<close>
   notes [fcomp_norm_unfold] = pointer_assn_def[symmetric]
 begin
 
 lemma ptr_update_code_rule:
   assumes \<open>nofail (f' ys a)\<close>
-  shows "llvm_htriple (pointer_assn R ys p \<and>* S a ai \<and>* \<up>\<^sub>dP ys a) (ptr_update_code f p ai)
+  shows "llvm_htriple (pointer_assn R ys p \<and>* S a ai \<and>* \<up>\<^sub>dP (ys, a)) (ptr_update_code f p ai)
     (\<lambda>r. (\<lambda>s. \<exists>xa xb. (pointer_assn R xa r \<and>*  \<up>(RETURN xa \<le> ptr_update f' ys a)) s) \<and>* \<box>)"
   (*supply [vcg_rules] = bpto_ptr_update_code2 does not work it looses track of dependencies between variables*)
   apply vcg
@@ -446,7 +692,7 @@ defer
   apply assumption
   by (simp add: STATE_extract(2) invalid_assn_def pure_true_conv)
 
-lemma ptr_update_hnr: \<open>(uncurry (ptr_update_code f), uncurry (ptr_update f')) \<in> [uncurry P]\<^sub>a (pointer_assn R)\<^sup>d *\<^sub>a S\<^sup>d \<rightarrow> pointer_assn R\<close>
+lemma ptr_update_hnr: \<open>(uncurry (ptr_update_code f), uncurry (ptr_update f')) \<in> [P]\<^sub>a (pointer_assn R)\<^sup>d *\<^sub>a S\<^sup>d \<rightarrow> pointer_assn R\<close>
   supply [vcg_rules] = ptr_update_code_rule
   apply sepref_to_hoare
   apply vcg
